formalization/BasicTyping.v
@@ -1,0 +1,124 @@
+From stdpp Require Import mapset.
+From CT Require Import CoreLangProp.
+
+Import Atom.
+Import CoreLang.
+Import Tactics.
+Import NamelessTactics.
+
+(** This file defines the basic type system of λᴱ. *)
+
+Definition ty_of_const (c: constant): base_ty :=
+  match c with
+  | cnat _ => TNat
+  | cbool _ => TBool
+  end.
+
+Definition ret_ty_of_op (op: op): base_ty :=
+  match op with
+  | op_plus_one => TNat
+  | op_minus_one => TNat
+  | op_eq_zero => TBool
+  | op_rannat => TNat
+  | op_ranbool => TBool
+  end.
+
+Definition ty_of_op (op: op): ty := TNat ⤍ (ret_ty_of_op op).
+
+Definition context := amap ty.
+#[global]
+Instance context_stale : Stale context := dom.
+Arguments context_stale /.
+
+Reserved Notation "Γ '⊢t' t '⋮t' T" (at level 40).
+Reserved Notation "Γ '⊢t' t '⋮v' T" (at level 40).
+
+(** Basic typing rules  *)
+Inductive tm_has_type : context -> tm -> ty -> Prop :=
+| BtValue : forall Γ v T, Γ ⊢t v ⋮v T -> Γ ⊢t v ⋮t T
+| BtLetE : forall Γ (e1 e2: tm) T1 T2 (L: aset),
+    Γ ⊢t e1 ⋮t T1 ->
+    (forall (x: atom), x ∉ L -> (<[ x := T1]> Γ) ⊢t e2 ^^^ x ⋮t T2) ->
+    Γ ⊢t (tlete e1 e2) ⋮t T2
+| BtEffOp : forall Γ (op: op) (v1: value) (e: tm) (T1 Tx: base_ty) T (L: aset),
+    Γ ⊢t v1 ⋮v T1 ->
+    (ty_of_op op) = T1 ⤍ Tx ->
+    (forall (x: atom), x ∉ L -> (<[x := TBase Tx]> Γ) ⊢t e ^^^ x ⋮t T) ->
+    Γ ⊢t tletop op v1 e ⋮t T
+| BtApp : forall Γ (v1 v2: value) (e: tm) T1 Tx T (L: aset),
+    Γ ⊢t v1 ⋮v T1 ⤍ Tx ->
+    Γ ⊢t v2 ⋮v T1 ->
+    (forall (x: atom), x ∉ L -> (<[x := Tx]> Γ) ⊢t e ^^^ x ⋮t T) ->
+    Γ ⊢t tletapp v1 v2 e ⋮t T
+| BtMatchb: forall Γ v e1 e2 T,
+    Γ ⊢t v ⋮v TBool ->
+    Γ ⊢t e1 ⋮t T ->
+    Γ ⊢t e2 ⋮t T ->
+    Γ ⊢t (tmatchb v e1 e2) ⋮t T
+with value_has_type : context -> value -> ty -> Prop :=
+| BtConst : forall Γ (c: constant), Γ ⊢t c ⋮v (ty_of_const c)
+| BtVar : forall Γ (x: atom) T,
+    Γ !! x = Some T -> Γ ⊢t x ⋮v T
+| BtFun : forall Γ Tx T (e: tm) (L: aset),
+    (forall (x: atom), x ∉ L -> (<[x := Tx]> Γ) ⊢t e ^^^ x ⋮t T) ->
+    Γ ⊢t vlam Tx e ⋮v Tx ⤍ T
+| BtFix : forall Γ (Tx: base_ty) T e (L: aset),
+    (forall (x: atom), x ∉ L -> (<[x := TBase Tx]>Γ) ⊢t (vlam (Tx ⤍ T) e) ^^^ x ⋮v ((Tx ⤍ T) ⤍ T)) ->
+    Γ ⊢t vfix (Tx ⤍ T) (vlam (Tx ⤍ T) e) ⋮v Tx ⤍ T
+where "Γ '⊢t' t '⋮t' T" := (tm_has_type Γ t T) and "Γ '⊢t' t '⋮v' T" := (value_has_type Γ t T).
+
+Scheme value_has_type_mutual_rec := Induction for value_has_type Sort Prop
+    with tm_has_type_mutual_rec := Induction for tm_has_type Sort Prop.
+
+Global Hint Constructors tm_has_type: core.
+Global Hint Constructors value_has_type: core.
+
+(** * Naming related properties of the basic type system *)
+
+Lemma basic_typing_contains_fv_tm: forall Γ e T, Γ ⊢t e ⋮t T -> fv_tm e ⊆ dom Γ
+with basic_typing_contains_fv_value: forall Γ e T, Γ ⊢t e ⋮v T -> fv_value e ⊆ dom Γ.
+Proof.
+  all:
+  destruct 1; simpl; eauto;
+  try select (forall x, _ ∉ _ -> _) (fun H => auto_pose_fv x; repeat specialize_with x);
+  repeat select (_ ⊢t _ ⋮v _) (fun H => apply basic_typing_contains_fv_value in H);
+  repeat select (_ ⊢t _ ⋮t _) (fun H => apply basic_typing_contains_fv_tm in H);
+  simpl in *;
+  repeat
+    match goal with
+    | H : fv_tm ({_ ~t> _} _) ⊆ _ |- _ =>
+        setoid_rewrite <- open_fv_tm' in H
+    | H : _ ⊆ dom (<[_:=_]>_) |- _ =>
+        setoid_rewrite dom_insert in H
+    | H : _ !! _ = _ |- _ =>
+        apply elem_of_dom_2 in H
+    end;
+  my_set_solver.
+Qed.
+
+Lemma basic_typing_closed_tm: forall e T, ∅ ⊢t e ⋮t T -> closed_tm e.
+Proof.
+  intros.
+  apply basic_typing_contains_fv_tm in H. my_set_solver.
+Qed.
+
+Lemma basic_typing_closed_value: forall v T, ∅ ⊢t v ⋮v T -> closed_value v.
+Proof.
+  intros.
+  apply basic_typing_contains_fv_value in H. my_set_solver.
+Qed.
+
+Lemma basic_typing_regular_value: forall Γ v t, Γ ⊢t v ⋮v t -> lc v
+with basic_typing_regular_tm: forall Γ e t, Γ ⊢t e ⋮t t -> lc e.
+Proof.
+  all: destruct 1; simpl;
+    try econstructor; try instantiate_atom_listctx; eauto.
+Qed.
+
+Ltac basic_typing_regular_simp :=
+  repeat match goal with
+    | [H: _ ⊢t _ ⋮v _ |- lc _] => apply basic_typing_regular_value in H; destruct H; auto
+    | [H: _ ⊢t _ ⋮t _ |- lc _] => apply basic_typing_regular_tm in H; destruct H; auto
+    | [H: _ ⊢t _ ⋮v _ |- body _] => apply basic_typing_regular_value in H; destruct H; auto
+    | [H: _ ⊢t _ ⋮t _ |- body _] => apply basic_typing_regular_tm in H; destruct H; auto
+    end.
