formalization/BasicTypingProp.v
@@ -1,0 +1,260 @@
+From stdpp Require Import mapset.
+From CT Require Import CoreLangProp.
+From CT Require Import BasicTyping.
+From CT Require Import OperationalSemantics.
+
+Import Atom.
+Import CoreLang.
+Import Tactics.
+Import NamelessTactics.
+Import BasicTyping.
+Import Trace.
+Import OperationalSemantics.
+
+(** This file proves properties of the basic type system. *)
+
+(** * Canonical forms *)
+
+Lemma basic_typing_bool_canonical_form: forall (v: value), ∅ ⊢t v ⋮v TBool -> v = true \/ v = false.
+Proof.
+  inversion 1; subst; simpl in *.
+  destruct c; simplify_eq. destruct b; eauto.
+  simplify_map_eq.
+Qed.
+
+Lemma basic_typing_nat_canonical_form: forall (v: value), ∅ ⊢t v ⋮v TNat -> (exists (i: nat), v = i).
+Proof.
+  inversion 1; subst; simpl in *.
+  destruct c; simplify_eq. eauto.
+  simplify_map_eq.
+Qed.
+
+Lemma basic_typing_base_canonical_form: forall (v: value) (B: base_ty), ∅ ⊢t v ⋮v B -> (exists (c: constant), v = c).
+Proof.
+  inversion 1; subst. eauto. simplify_map_eq.
+Qed.
+
+Lemma basic_typing_arrow_canonical_form:
+  forall (v: value) T1 T2, ∅ ⊢t v ⋮v T1 ⤍ T2 ->
+                      (exists e, v = vlam T1 e) \/ (exists e, v = vfix (T1 ⤍ T2) (vlam (T1 ⤍ T2) e)).
+Proof.
+  inversion 1; subst. simplify_map_eq.
+  - left. eauto.
+  - right. eexists. f_equal.
+Qed.
+
+
+(** * Weakening lemmas *)
+
+Lemma basic_typing_weaken_tm: forall Γ Γ' (v: tm) T,
+    Γ ⊆ Γ' -> Γ ⊢t v ⋮t T -> Γ' ⊢t v ⋮t T
+with basic_typing_weaken_value: forall Γ Γ' (v: value) T,
+    Γ ⊆ Γ' -> Γ ⊢t v ⋮v T -> Γ' ⊢t v ⋮v T.
+Proof.
+  all : intros * Hs; destruct 1; econstructor; eauto using lookup_weaken.
+  all: instantiate_atom_listctx;
+    auto_eapply;
+    try lazymatch goal with
+      | |- _ ⊆ _ => apply insert_mono; eauto
+      | _ => eauto
+      end.
+Qed.
+
+Lemma basic_typing_weaken_insert_tm: forall Γ (v: tm) T x U,
+    x # Γ -> Γ ⊢t v ⋮t T -> <[x := U]>Γ ⊢t v ⋮t T.
+Proof.
+  intros. eapply basic_typing_weaken_tm. 2: eauto.
+  apply insert_subseteq. apply not_elem_of_dom. my_set_solver.
+Qed.
+
+Lemma basic_typing_weaken_insert_value: forall Γ (v: value) T x U,
+    x # Γ -> Γ ⊢t v ⋮v T -> <[x := U]> Γ ⊢t v ⋮v T.
+Proof.
+  intros. eapply basic_typing_weaken_value. 2: eauto.
+  apply insert_subseteq. apply not_elem_of_dom. my_set_solver.
+Qed.
+
+(** * Substitution lemmas *)
+
+Lemma basic_typing_subst_tm: forall Γ z u U (v: tm) T, Γ ⊢t u ⋮v U -> <[z := U]> Γ ⊢t v ⋮t T -> Γ ⊢t {z := u}t v ⋮t T.
+Proof.
+  intros * Hu Ht; remember (<[z:=U]> Γ) as Γ'; generalize dependent Γ.
+  revert Γ' v T Ht.
+  apply (tm_has_type_mutual_rec
+           (fun c v T _ => ∀ Γ, Γ ⊢t u ⋮v U → c = <[z:=U]> Γ → Γ ⊢t {z := u }v v ⋮v T)
+           (fun c v T _ => ∀ Γ, Γ ⊢t u ⋮v U → c = <[z:=U]> Γ → Γ ⊢t {z := u }t v ⋮t T));
+  (* [context] should be defined as a notation which helps resolving typeclass
+  instances for, e.g., rewriting. *)
+    unfold context;
+    intros; subst; simpl in *; eauto; try econstructor; eauto.
+  case_decide; subst.
+  by simplify_map_eq.
+  econstructor. by simplify_map_eq.
+
+  all:
+  instantiate_atom_listctx;
+  rewrite <- subst_open_var_tm by
+    (eauto using basic_typing_regular_value; my_set_solver);
+  auto_eapply; [
+      eapply basic_typing_weaken_insert_value; eauto; my_set_solver
+    | apply insert_commute; my_set_solver ].
+Qed.
+
+Lemma basic_typing_subst_value: forall Γ z u U (v: value) T, Γ ⊢t u ⋮v U -> <[z := U]> Γ ⊢t v ⋮v T -> Γ ⊢t {z := u}v v ⋮v T.
+Proof.
+  intros * Hu Ht; remember (<[z:=U]> Γ) as Γ'; generalize dependent Γ.
+  revert Γ' v T Ht.
+  apply (value_has_type_mutual_rec
+           (fun c v T _ => ∀ Γ, Γ ⊢t u ⋮v U → c = <[z:=U]> Γ → Γ ⊢t {z := u }v v ⋮v T)
+           (fun c v T _ => ∀ Γ, Γ ⊢t u ⋮v U → c = <[z:=U]> Γ → Γ ⊢t {z := u }t v ⋮t T));
+    unfold context;
+    intros; subst; simpl in *; eauto; try econstructor; eauto.
+  case_decide; subst.
+  by simplify_map_eq.
+  econstructor. by simplify_map_eq.
+
+  all:
+  instantiate_atom_listctx;
+  rewrite <- subst_open_var_tm by
+    (eauto using basic_typing_regular_value; my_set_solver);
+  auto_eapply; [
+      eapply basic_typing_weaken_insert_value; eauto; my_set_solver
+    | apply insert_commute; my_set_solver ].
+Qed.
+
+(** * Type uniqueness lemmas *)
+
+Lemma basic_typing_tm_unique: forall Γ e T1 T2,
+    Γ ⊢t e ⋮t T1 ->
+    Γ ⊢t e ⋮t T2 ->
+    T1 = T2.
+Proof.
+  intros * H. revert T2. revert_all.
+  apply (tm_has_type_mutual_rec
+           (fun Γ v T1 _ => ∀ T2, Γ ⊢t v ⋮v T2 → T1 = T2)
+           (fun Γ e T1 _ => ∀ T2, Γ ⊢t e ⋮t T2 → T1 = T2));
+    intros;
+    try match goal with
+      | H : _ ⊢t _ ⋮t _ |- _ => sinvert H
+      | H : _ ⊢t _ ⋮v _ |- _ => sinvert H
+      end; eauto;
+    try solve [ auto_pose_fv x; repeat specialize_with x; hauto ].
+  by simplify_map_eq.
+Qed.
+
+Lemma basic_typing_value_unique: forall Γ v T1 T2,
+    Γ ⊢t v ⋮v T1 ->
+    Γ ⊢t v ⋮v T2 ->
+    T1 = T2.
+Proof.
+  intros * H. revert T2. revert_all.
+  apply (value_has_type_mutual_rec
+           (fun Γ v T1 _ => ∀ T2, Γ ⊢t v ⋮v T2 → T1 = T2)
+           (fun Γ e T1 _ => ∀ T2, Γ ⊢t e ⋮t T2 → T1 = T2));
+    intros;
+    try match goal with
+      | H : _ ⊢t _ ⋮t _ |- _ => sinvert H
+      | H : _ ⊢t _ ⋮v _ |- _ => sinvert H
+      end; eauto;
+    try solve [ auto_pose_fv x; repeat specialize_with x; hauto ].
+  by simplify_map_eq.
+Qed.
+
+(** * Strengthening lemmas *)
+
+(* This statement can be generalized to taking a union of the context and a
+disjoint new context. *)
+Lemma basic_typing_strengthen_tm: forall Γ x Tx (v: tm) T,
+    (<[x:=Tx]>Γ) ⊢t v ⋮t T -> x # v -> Γ ⊢t v ⋮t T
+with basic_typing_strengthen_value: forall Γ x Tx (v: value) T,
+    (<[x:=Tx]>Γ) ⊢t v ⋮v T -> x # v -> Γ ⊢t v ⋮v T.
+Proof.
+  all : intros * H Hfresh; remember (<[x:=Tx]>Γ);
+    generalize dependent Γ;
+    destruct H; intros; unfold context in *; subst;
+    econstructor; eauto;
+    try solve [
+        try instantiate_atom_listctx;
+        try rewrite insert_commute in * by my_set_solver;
+        auto_eapply; eauto;
+        match goal with
+        | |- context [{_ ~t> _} _] =>
+            eapply not_elem_of_weaken; [ | apply open_fv_tm ]; my_set_solver
+        | _ => my_set_solver
+        end ].
+  by rewrite lookup_insert_ne in * by my_set_solver.
+Qed.
+
+(** * Type properties of syntax sugar *)
+
+Lemma mk_app_e_v_has_type Γ e v T1 T2 :
+  Γ ⊢t e ⋮t T1 ⤍ T2 ->
+  Γ ⊢t v ⋮v T1 ->
+  Γ ⊢t mk_app_e_v e v ⋮t T2.
+Proof.
+  intros.
+  econstructor; eauto.
+  instantiate_atom_listctx.
+  simpl. econstructor. econstructor. simplify_map_eq. reflexivity.
+  rewrite open_rec_lc_value by eauto using basic_typing_regular_value.
+  apply basic_typing_weaken_insert_value; eauto. my_set_solver.
+  simpl. instantiate_atom_listctx. econstructor. econstructor. simplify_map_eq.
+  reflexivity.
+Qed.
+
+Lemma mk_app_e_v_has_type_inv Γ e v T2 :
+  Γ ⊢t mk_app_e_v e v ⋮t T2 ->
+  lc v ->
+  exists T1, Γ ⊢t e ⋮t T1 ⤍ T2 /\ Γ ⊢t v ⋮v T1.
+Proof.
+  intros.
+  sinvert H.
+  simpl in H6.
+  auto_pose_fv x. repeat specialize_with x.
+  rewrite open_rec_lc_value in H6 by auto.
+  sinvert H6. simpl in H10.
+  auto_pose_fv y. repeat specialize_with y.
+  sinvert H7. setoid_rewrite lookup_insert in H5. simplify_eq.
+  sinvert H10. sinvert H5. setoid_rewrite lookup_insert in H6. simplify_eq.
+  repeat esplit; eauto.
+  eapply basic_typing_strengthen_value; eauto. my_set_solver.
+Qed.
+
+(** * Type preservation *)
+
+Lemma tr_reduction_sound α op c1 c :
+  α⊧{op~c1}⇓{c} ->
+  ty_of_const c = ret_ty_of_op op.
+Proof.
+  induction 1; eauto.
+Qed.
+
+(** perservation *)
+Lemma preservation: forall α β Γ T (e e': tm),α ⊧ e ↪{ β } e' -> Γ ⊢t e ⋮t T -> Γ ⊢t e' ⋮t T.
+Proof.
+  intros * Hstep HT. move HT at top. revert_all.
+  induction 1; intros; sinvert Hstep; eauto.
+  - auto_pose_fv x. repeat specialize_with x.
+    rewrite <- subst_intro_tm with (x:=x) by (eauto; my_set_solver).
+    sinvert HT. eauto using basic_typing_subst_tm.
+  - auto_pose_fv x. repeat specialize_with x.
+    rewrite <- subst_intro_tm with (x:=x) by (eauto; my_set_solver).
+    sinvert H0. erewrite <- tr_reduction_sound in H1; eauto.
+    eauto using basic_typing_subst_tm.
+  - sinvert H.
+    econstructor; eauto.
+    auto_pose_fv x. repeat specialize_with x.
+    rewrite <- subst_intro_tm with (x:=x) by (eauto; my_set_solver).
+    eauto using basic_typing_subst_tm.
+  - sinvert H.
+    econstructor; eauto.
+    auto_pose_fv x. repeat specialize_with x.
+    rewrite <- subst_intro_value with (x:=x) by (eauto; my_set_solver).
+    eauto using basic_typing_subst_value.
+Qed.
+
+(** multi preservation *)
+Lemma multi_preservation: forall α β Γ T (e e': tm),α ⊧ e ↪*{ β } e' -> Γ ⊢t e ⋮t T -> Γ ⊢t e' ⋮t T.
+Proof.
+  induction 1; eauto using preservation.
+Qed.
